F_mu_ref_par/fundamental_binary.v
@@ -4,7 +4,7 @@ From iris_logrel.F_mu_ref_par Require Import rules_binary.
 From iris.algebra Require Export upred_big_op.
 
 Section typed_interp.
-  Context `{heapIG Σ, cfgSG Σ} (N : namespace).
+  Context `{heapIG Σ, cfgSG Σ}.
   Notation D := (prodC valC valC -n> iPropG lang Σ).
   Implicit Types e : expr.
   Implicit Types Δ : listC D.
@@ -24,11 +24,10 @@ Section typed_interp.
   Definition bin_log_related (Δ : listC D) (Γ : list type)
       (e e' : expr) (τ : type) : Prop := ∀ vvs ρ j K,
     length Γ = length vvs →
-    heapI_ctx (N .@ 2) ★ Spec_ctx (N .@ 3) ρ ★
-      [∧] zip_with (λ τ, interp (N .@ 1) τ Δ) Γ vvs ★
-      j ⤇ fill K (e'.[env_subst (map snd vvs)])
+    heapI_ctx ★ spec_ctx ρ ★ [∧] zip_with (λ τ, interp τ Δ) Γ vvs ★
+      j ⤇ fill K (e'.[env_subst (vvs.*2)])
     ⊢ WP e.[env_subst (vvs.*1)] {{ v, ∃ v',
-        j ⤇ fill K (# v') ★ interp (N .@ 1) τ Δ (v, v') }}.
+        j ⤇ fill K (# v') ★ interp τ Δ (v, v') }}.
 
   Notation "Δ ∥ Γ ⊩ e '≤log≤' e' ∷ τ" := (bin_log_related Δ Γ e e' τ)
                                        (at level 20).
@@ -56,7 +55,7 @@ Section typed_interp.
     iIntros {vvs ρ j K Hlen} "(#Hh & #Hs & #HΓ & Hj) /=".
     smart_wp_bind (FstCtx) v v' "[Hv #Hiv]" (IHHtyped _ _ j (K ++ [FstCtx])); cbn.
     iDestruct "Hiv" as { [w1 w1'] [w2 w2'] } "#[% [Hw1 Hw2]]"; simplify_eq.
-    iPvs (step_fst (N .@ 3) _ _ j K (# w1') w1' (# w2') w2' with "* [-]") as "Hw"; eauto.
+    iPvs (step_fst _ _ j K (# w1') w1' (# w2') w2' with "* [-]") as "Hw"; eauto.
     iApply wp_fst; eauto.
   Qed.
 
@@ -67,7 +66,7 @@ Section typed_interp.
     iIntros {vvs ρ j K Hlen} "(#Hh & #Hs & #HΓ & Hj) /=".
     smart_wp_bind (SndCtx) v v' "[Hv #Hiv]" (IHHtyped _ _ j (K ++ [SndCtx])); cbn.
     iDestruct "Hiv" as { [w1 w1'] [w2 w2'] } "#[% [Hw1 Hw2]]"; simplify_eq.
-    iPvs (step_snd (N .@ 3) _ _ j K (# w1') w1' (# w2') w2' with "* [-]") as "Hw"; eauto.
+    iPvs (step_snd _ _ j K (# w1') w1' (# w2') w2' with "* [-]") as "Hw"; eauto.
     iApply wp_snd; eauto.
   Qed.
 
@@ -108,14 +107,14 @@ Section typed_interp.
       (IHHtyped1 _ _ j (K ++ [CaseCtx _ _])); cbn.
     iDestruct "Hiv" as "[Hiv|Hiv]".
     - iDestruct "Hiv" as { [w w'] } "[% Hw]"; simplify_eq.
-      iPvs (step_case_inl (N .@ 3) _ _ j K (# w') w' with "* [-]") as "Hz"; eauto.
+      iPvs (step_case_inl _ _ j K (# w') w' with "* [-]") as "Hz"; eauto.
       iApply wp_case_inl; auto 1 using to_of_val; asimpl.
       specialize (IHHtyped2 ((w,w') :: vvs)); cbn in IHHtyped2.
       erewrite <- ?n_closed_subst_head_simpl in IHHtyped2; eauto;
         simpl; try rewrite fmap_length; eauto with f_equal.
       iNext. iApply IHHtyped2; eauto.
     - iDestruct "Hiv" as { [w w'] } "[% Hw]"; simplify_eq.
-      iPvs (step_case_inr (N .@ 3) _ _ j K (# w') w' with "* [-]") as "Hz"; eauto.
+      iPvs (step_case_inr _ _ j K (# w') w' with "* [-]") as "Hz"; eauto.
       iApply wp_case_inr; auto 1 using to_of_val; asimpl.
       specialize (IHHtyped3 ((w,w') :: vvs)); cbn in IHHtyped3.
       erewrite <- ?n_closed_subst_head_simpl in IHHtyped3; eauto;
@@ -133,9 +132,9 @@ Section typed_interp.
     smart_wp_bind (IfCtx _ _) v v' "[Hv #Hiv]"
       (IHHtyped1 _ _ j (K ++ [IfCtx _ _])); cbn.
     iDestruct "Hiv" as { [] } "[% %]"; simplify_eq/=.
-    - iPvs (step_if_true (N .@ 3) _ _ j K with "* [-]") as "Hz"; eauto.
+    - iPvs (step_if_true _ _ j K with "* [-]") as "Hz"; eauto.
       iApply wp_if_true. iNext. iApply IHHtyped2; eauto.
-    - iPvs (step_if_false (N .@ 3) _ _ j K with "* [-]") as "Hz"; eauto.
+    - iPvs (step_if_false _ _ j K with "* [-]") as "Hz"; eauto.
       iApply wp_if_false. iNext. iApply IHHtyped3; eauto.
   Qed.
 
@@ -151,7 +150,7 @@ Section typed_interp.
                   (IHHtyped2 _ _ j (K ++ [BinOpRCtx _ _])); cbn.
     iDestruct "Hiv" as {n} "[% %]"; simplify_eq/=.
     iDestruct "Hiw" as {n'} "[% %]"; simplify_eq/=.
-    iPvs (step_nat_bin_op (N .@ 3) _ _ j K with "* [-]") as "Hz"; eauto.
+    iPvs (step_nat_bin_op _ _ j K with "* [-]") as "Hz"; eauto.
     iApply wp_nat_bin_op. iNext. iPvsIntro. iExists _; iSplitL; eauto.
     destruct op; simpl; try destruct eq_nat_dec; try destruct le_dec;
       try destruct lt_dec; eauto.
@@ -167,7 +166,7 @@ Section typed_interp.
     value_case. iExists (LamV _). iIntros "{$Hj} !".
     iLöb as "IH". iIntros {j' K' [v v'] } "[#Hiv Hv]".
     iApply wp_lam; auto 1 using to_of_val. iNext.
-    iPvs (step_lam (N .@ 3) _ _ j' K' _ (# v') v' with "* [-]") as "Hz"; eauto.
+    iPvs (step_lam _ _ j' K' _ (# v') v' with "* [-]") as "Hz"; eauto.
     asimpl.
     specialize (IHHtyped ((LamV e.[upn 2 (env_subst (vvs.*1))],
       LamV e'.[upn 2 (env_subst (vvs.*2))]) :: (v,v') :: vvs)); cbn in IHHtyped.
@@ -198,7 +197,7 @@ Section typed_interp.
     value_case. iExists (TLamV _).
     iIntros "{$Hj} /= !"; iIntros {τi j' K'} "% Hv /=".
     iApply wp_TLam; iNext.
-    iPvs (step_Tlam (N .@ 3) _ _ j' K' (e'.[env_subst (vvs.*2)]) with "* [-]")
+    iPvs (step_Tlam _ _ j' K' (e'.[env_subst (vvs.*2)]) with "* [-]")
       as "Hz"; eauto.
     iApply IHHtyped; [by rewrite fmap_length|].
     iFrame "Hh Hs Hz". rewrite zip_with_fmap_l. by iApply context_interp_ren_S.
@@ -212,7 +211,7 @@ Section typed_interp.
     smart_wp_bind (TAppCtx) v v' "[Hj #Hv]"
       (IHHtyped _ _ j (K ++ [TAppCtx])); cbn.
     iApply wp_wand_r; iSplitL.
-    { iApply ("Hv" $! (interp (N .@ 1) τ' Δ) with "[#] Hj"); iPureIntro; apply _. }
+    { iApply ("Hv" $! (interp τ' Δ) with "[#] Hj"); iPureIntro; apply _. }
     iIntros {w} "Hw". iDestruct "Hw" as {w'} "[Hw #Hiw]".
     iExists _; rewrite -interp_subst; eauto.
   Qed.
@@ -243,9 +242,9 @@ Section typed_interp.
           rewrite ?fill_app; simpl; repeat iSplitR; trivial].
     iIntros {v}. iDestruct 1 as {v'} "[Hw #Hiw]"; rewrite fill_app.
     rewrite /= fixpoint_unfold /=.
-    change (fixpoint _) with (@interp _ _ _ (N .@ 1) (TRec τ) Δ).
+    change (fixpoint _) with (interp (TRec τ) Δ).
     iDestruct "Hiw" as { [w w'] } "#[% Hiz]"; simplify_eq/=.
-    iPvs (step_Fold _ _ _ j K (# w') w' with "* [-]") as "Hz"; eauto.
+    iPvs (step_Fold _ _ j K (# w') w' with "* [-]") as "Hz"; eauto.
     iApply wp_Fold; cbn; auto.
     iNext; iPvsIntro; iExists _; iFrame "Hz". by rewrite -interp_subst.
   Qed.
@@ -255,7 +254,7 @@ Section typed_interp.
     Δ ∥ Γ ⊩ Fork e ≤log≤ Fork e' ∷ TUnit.
   Proof.
     iIntros {vvs ρ j K Hlen} "(#Hh & #Hs & #HΓ & Hj) /=".
-    iPvs (step_fork (N .@ 3) _ _ j K with "* [-]") as {j'} "[Hj Hj']"; eauto.
+    iPvs (step_fork _ _ j K with "* [-]") as {j'} "[Hj Hj']"; eauto.
     iApply wp_fork; iNext; iSplitL "Hj".
     - iExists UnitV; eauto.
     - iApply wp_wand_l; iSplitR; [|iApply (IHHtyped _ _ _ [])]; eauto.
@@ -267,11 +266,11 @@ Section typed_interp.
   Proof.
     iIntros {vvs ρ j K Hlen} "(#Hh & #Hs & #HΓ & Hj) /=".
     smart_wp_bind (AllocCtx) v v' "[Hv #Hiv]" (IHHtyped _ _ j (K ++ [AllocCtx])).
-    iPvs (step_alloc (N .@ 3) _ _ j K (# v') v' with "* [-]") as {l'} "[Hj Hl]"; eauto.
+    iPvs (step_alloc _ _ j K (# v') v' with "* [-]") as {l'} "[Hj Hl]"; eauto.
     iApply wp_alloc; auto.
     iIntros "{$Hh} >"; iIntros {l} "Hl'".
-    iPvs (inv_alloc (N .@ 1 .@ (l,l')) _ (∃ w : val * val,
-      l ↦ᵢ w.1 ★ l' ↦ₛ w.2 ★ interp (N .@ 1) τ Δ w)%I with "[Hl Hl']") as "HN"; eauto.
+    iPvs (inv_alloc (logN .@ (l,l')) _ (∃ w : val * val,
+      l ↦ᵢ w.1 ★ l' ↦ₛ w.2 ★ interp τ Δ w)%I with "[Hl Hl']") as "HN"; eauto.
     { iNext; iExists (v, v'); by iFrame. }
     iPvsIntro; iExists (LocV l'). iFrame "Hj". iExists (l, l'); eauto.
   Qed.
@@ -283,11 +282,11 @@ Section typed_interp.
     iIntros {vvs ρ j K Hlen} "(#Hh & #Hs & #HΓ & Hj) /=".
     smart_wp_bind (LoadCtx) v v' "[Hv #Hiv]" (IHHtyped _ _ j (K ++ [LoadCtx])).
     iDestruct "Hiv" as { [l l'] } "[% Hinv]"; simplify_eq/=.
-    iInv (N .@ 1 .@ (l,l')) as { [w w'] } "[Hw1 [Hw2 #Hw]]"; simpl.
+    iInv (logN .@ (l,l')) as { [w w'] } "[Hw1 [Hw2 #Hw]]"; simpl.
     iTimeless "Hw2".
-    iPvs (step_load (N .@ 3) _ _ j K l' 1 w' with "[Hv Hw2]") as "[Hv Hw2]";
+    iPvs (step_load _ _ j K l' 1 w' with "[Hv Hw2]") as "[Hv Hw2]";
       [solve_ndisj|by iFrame|].
-    iApply (wp_load _ _ _ 1); [|iFrame "Hh"]; trivial; try solve_ndisj.
+    iApply (wp_load _ _ 1); [|iFrame "Hh"]; trivial; try solve_ndisj.
     iIntros "{$Hw1} > Hw1". iPvsIntro. iSplitL "Hw1 Hw2".
     - iNext; iExists (w,w'); by iFrame.
     - iExists w'; by iFrame.
@@ -304,12 +303,12 @@ Section typed_interp.
     smart_wp_bind (StoreRCtx _) w w' "[Hw #Hiw]"
       (IHHtyped2 _ _ j (K ++ [StoreRCtx _])).
     iDestruct "Hiv" as { [l l'] } "[% Hinv]"; simplify_eq/=.
-    iInv (N .@ 1 .@ (l,l')) as { [v v'] } "[Hv1 [Hv2 #Hv]]".
+    iInv (logN .@ (l,l')) as { [v v'] } "[Hv1 [Hv2 #Hv]]".
     { eapply bool_decide_spec; eauto using to_of_val. }
     iTimeless "Hv2".
-    iPvs (step_store (N .@ 3) _ _ j K l' v' (# w') w' with "[Hw Hv2]")
+    iPvs (step_store _ _ j K l' v' (# w') w' with "[Hw Hv2]")
       as "[Hw Hv2]"; [eauto|solve_ndisj|by iFrame|].
-    iApply (wp_store (N .@ 2)); auto using to_of_val. solve_ndisj.
+    iApply wp_store; auto using to_of_val. solve_ndisj.
     iIntros "{$Hh $Hv1} > Hv1". iPvsIntro. iSplitL "Hv1 Hv2".
     - iNext; iExists (w, w'); by iFrame.
     - iExists UnitV; iFrame; auto.
@@ -330,23 +329,23 @@ Section typed_interp.
     smart_wp_bind (CasRCtx _ _) u u' "[Hu #Hiu]"
       (IHHtyped3 _ _ j (K ++ [CasRCtx _ _])).
     iDestruct "Hiv" as { [l l'] } "[% Hinv]"; simplify_eq/=.
-    iInv (N .@ 1 .@ (l,l')) as { [v v'] } "[Hv1 [Hv2 #Hv]]".
+    iInv (logN .@ (l,l')) as { [v v'] } "[Hv1 [Hv2 #Hv]]".
     { eapply bool_decide_spec; eauto 10 using to_of_val. }
     iTimeless "Hv2".
     destruct (decide (v = w)) as [|Hneq]; subst.
-    - iPvs (step_cas_suc (N .@ 3) _ _ j K l' (# w') w' v' (# u') u'
+    - iPvs (step_cas_suc _ _ j K l' (# w') w' v' (# u') u'
             with "[Hu Hv2]") as "[Hw Hv2]"; simpl; eauto; first solve_ndisj.
       { iIntros "{$Hs $Hu $Hv2} >".
         rewrite ?interp_EqType_agree; trivial. by iSimplifyEq. }
-      iApply (wp_cas_suc (N .@ 2)); eauto using to_of_val; first solve_ndisj.
+      iApply wp_cas_suc; eauto using to_of_val; first solve_ndisj.
       iIntros "{$Hh $Hv1} > Hv1". iPvsIntro. iSplitL "Hv1 Hv2".
       + iNext; iExists (_, _); by iFrame.
       + iExists (♭v true); iFrame; eauto.
-    - iPvs (step_cas_fail (N .@ 3) _ _ j K l' 1 v' (# w') w' (# u') u'
+    - iPvs (step_cas_fail _ _ j K l' 1 v' (# w') w' (# u') u'
             with "[Hu Hv2]") as "[Hw Hv2]"; simpl; eauto; first solve_ndisj.
       { iIntros "{$Hs $Hu $Hv2} >".
         rewrite ?interp_EqType_agree; trivial. by iSimplifyEq. }
-      iApply (wp_cas_fail (N .@ 2)); eauto using to_of_val; first solve_ndisj.
+      iApply wp_cas_fail; eauto using to_of_val; first solve_ndisj.
       iIntros "{$Hh $Hv1} > Hv1". iPvsIntro. iSplitL "Hv1 Hv2".
       + iNext; iExists (_, _); by iFrame.
       + iExists (♭v false); eauto.
