F_mu_ref_par/examples/lock.v
@@ -74,33 +74,33 @@ Proof.
 Qed.
 
 Section proof.
-  Context {Σ : gFunctors} {iS : cfgSG Σ}.
+  Context `{cfgSG Σ}.
 
-  Lemma steps_newlock N E ρ j K :
-    nclose N ⊆ E →
-    Spec_ctx N ρ ★ j ⤇ fill K newlock
+  Lemma steps_newlock E ρ j K :
+    nclose specN ⊆ E →
+    spec_ctx ρ ★ j ⤇ fill K newlock
       ={E}=> ∃ l, j ⤇ fill K (Loc l) ★ l ↦ₛ (♭v false).
   Proof.
     iIntros {HNE} "[#Hspec Hj]".
-    by iPvs (step_alloc _ _ _ j K with "[Hj]") as "Hj"; eauto.
+    by iPvs (step_alloc _ _ j K with "[Hj]") as "Hj"; eauto.
   Qed.
 
   Global Opaque newlock.
 
-  Lemma steps_acquire N E ρ j K l :
-    nclose N ⊆ E →
-    Spec_ctx N ρ ★ l ↦ₛ (♭v false) ★ j ⤇ fill K (App acquire (Loc l))
+  Lemma steps_acquire E ρ j K l :
+    nclose specN ⊆ E →
+    spec_ctx ρ ★ l ↦ₛ (♭v false) ★ j ⤇ fill K (App acquire (Loc l))
       ={E}=> j ⤇ fill K Unit ★ l ↦ₛ (♭v true).
   Proof.
     iIntros {HNE} "[#Hspec [Hl Hj]]". unfold acquire.
-    iPvs (step_lam _ _ _ j K with "[Hj]") as "Hj"; eauto. done.
-    iPvs (step_cas_suc _ _ _ j (K ++ [IfCtx _ _])
+    iPvs (step_lam _ _ j K with "[Hj]") as "Hj"; eauto. done.
+    iPvs (step_cas_suc _ _ j (K ++ [IfCtx _ _])
                        _ _ _ _ _ _ _ _ _ with "[Hj Hl]") as "[Hj Hl]"; trivial.
     rewrite ?fill_app. simpl.
     iFrame "Hspec Hj Hl"; trivial.
     iNext; trivial.
     rewrite ?fill_app. simpl.
-    iPvs (step_if_true _ _ _ j K _ _ _ with "[Hj]") as "Hj"; trivial.
+    iPvs (step_if_true _ _ j K _ _ _ with "[Hj]") as "Hj"; trivial.
     iFrame "Hspec Hj"; trivial.
     iPvsIntro. iFrame "Hj Hl"; trivial.
     Unshelve. all:trivial.
@@ -108,14 +108,14 @@ Section proof.
 
   Global Opaque acquire.
 
-  Lemma steps_release N E ρ j K l b:
-    nclose N ⊆ E →
-    Spec_ctx N ρ ★ l ↦ₛ (♭v b) ★ j ⤇ fill K (App release (Loc l))
+  Lemma steps_release E ρ j K l b:
+    nclose specN ⊆ E →
+    spec_ctx ρ ★ l ↦ₛ (♭v b) ★ j ⤇ fill K (App release (Loc l))
       ={E}=> j ⤇ fill K Unit ★ l ↦ₛ (♭v false).
   Proof.
     iIntros {HNE} "[#Hspec [Hl Hj]]". unfold release.
-    iPvs (step_lam _ _ _ j K with "[Hj]") as "Hj"; eauto; try done.
-    iPvs (step_store _ _ _ j K _ _ _ _ _ with "[Hj Hl]") as "[Hj Hl]"; eauto.
+    iPvs (step_lam _ _ j K with "[Hj]") as "Hj"; eauto; try done.
+    iPvs (step_store _ _ j K _ _ _ _ _ with "[Hj Hl]") as "[Hj Hl]"; eauto.
     iFrame "Hspec Hj"; trivial.
     iPvsIntro. iFrame "Hj Hl"; trivial.
     Unshelve. all: trivial.
@@ -123,36 +123,36 @@ Section proof.
 
   Global Opaque release.
 
-  Lemma steps_with_lock N E ρ j K e l P Q v w:
-    nclose N ⊆ E →
+  Lemma steps_with_lock E ρ j K e l P Q v w:
+    nclose specN ⊆ E →
     (∀ f, e.[f] = e) (* e is a closed term *) →
-    (∀ K', Spec_ctx N ρ ★ P ★ j ⤇ fill K' (App e (# w))
+    (∀ K', spec_ctx ρ ★ P ★ j ⤇ fill K' (App e (# w))
             ={E}=> j ⤇ fill K' (# v) ★ Q) →
-    Spec_ctx N ρ ★ P ★ l ↦ₛ (♭v false)
+    spec_ctx ρ ★ P ★ l ↦ₛ (♭v false)
                 ★ j ⤇ fill K (App (with_lock e (Loc l)) (# w))
       ={E}=> j ⤇ fill K (# v) ★ Q ★ l ↦ₛ (♭v false).
   Proof.
     iIntros {HNE H1 H2} "[#Hspec [HP [Hl Hj]]]".
-    iPvs (step_lam _ _ _ j K _ _ _ _ with "[Hj]") as "Hj"; eauto.
+    iPvs (step_lam _ _ j K _ _ _ _ with "[Hj]") as "Hj"; eauto.
     asimpl. rewrite H1.
-    iPvs (steps_acquire _ _ _ j (K ++ [AppRCtx (LamV _)])
+    iPvs (steps_acquire _ _ j (K ++ [AppRCtx (LamV _)])
                    _ _ with "[Hj Hl]") as "[Hj Hl]"; eauto.
     rewrite fill_app; simpl.
     iFrame "Hspec Hj"; trivial.
     rewrite fill_app; simpl.
-    iPvs (step_lam _ _ _ j K _ _ _ _ with "[Hj]") as "Hj"; eauto.
+    iPvs (step_lam _ _ j K _ _ _ _ with "[Hj]") as "Hj"; eauto.
     asimpl. rewrite H1.
     iPvs (H2 (K ++ [AppRCtx (LamV _)]) with "[Hj HP]") as "[Hj HQ]"; eauto.
     rewrite ?fill_app /=.
     iFrame "Hspec HP"; trivial.
     rewrite ?fill_app /=.
-    iPvs (step_lam _ _ _ j K _ _ _ _ with "[Hj]") as "Hj"; eauto.
+    iPvs (step_lam _ _ j K _ _ _ _ with "[Hj]") as "Hj"; eauto.
     asimpl.
-    iPvs (steps_release _ _ _ j (K ++ [AppRCtx (LamV _)]) _ _ with "[Hj Hl]")
+    iPvs (steps_release _ _ j (K ++ [AppRCtx (LamV _)]) _ _ with "[Hj Hl]")
       as "[Hj Hl]"; eauto.
     rewrite ?fill_app /=. by iFrame.
     rewrite ?fill_app /=.
-    iPvs (step_lam _ _ _ j K _ _ _ _ with "[Hj]") as "Hj"; eauto.
+    iPvs (step_lam _ _ j K _ _ _ _ with "[Hj]") as "Hj"; eauto.
     asimpl. iPvsIntro; by iFrame.
     Unshelve.
     all: try match goal with |- to_val _ = _ => auto using to_of_val end.
