F_mu_ref_par/examples/stack/CG_stack.v
@@ -57,7 +57,7 @@ Definition CG_stack : expr :=
                 (Alloc (Fold (InjL Unit))))) newlock).
 
 Section CG_Stack.
-  Context {Σ : gFunctors} {iS : cfgSG Σ}.
+  Context `{cfgSG Σ}.
 
   Lemma CG_push_type st Γ τ :
     typed Γ st (Tref (CG_StackType τ)) →
@@ -71,26 +71,26 @@ Section CG_Stack.
 
   Lemma CG_push_closed (st : expr) :
     (∀ f, st.[f] = st) → ∀ f, (CG_push st).[f] = CG_push st.
-  Proof. intros H f. unfold CG_push. asimpl. rewrite ?H; trivial. Qed.
+  Proof. intros Hst f. unfold CG_push. asimpl. rewrite ?Hst; trivial. Qed.
 
   Lemma CG_push_subst (st : expr) f : (CG_push st).[f] = CG_push st.[f].
   Proof. unfold CG_push; asimpl; trivial. Qed.
 
-  Lemma steps_CG_push N E ρ j K st v w :
-    nclose N ⊆ E →
-    Spec_ctx N ρ ★ st ↦ₛ v ★ j ⤇ fill K (App (CG_push (Loc st)) (# w))
+  Lemma steps_CG_push E ρ j K st v w :
+    nclose specN ⊆ E →
+    spec_ctx ρ ★ st ↦ₛ v ★ j ⤇ fill K (App (CG_push (Loc st)) (# w))
     ={E}=> j ⤇ fill K Unit ★ st ↦ₛ FoldV (InjRV (PairV w v)).
   Proof.
     intros HNE. iIntros "[#Hspec [Hx Hj]]". unfold CG_push.
-    iPvs (step_lam _ _ _ j K _ _ _ _ with "[Hj]") as "Hj"; eauto.
+    iPvs (step_lam _ _ j K _ _ _ _ with "[Hj]") as "Hj"; eauto.
     asimpl.
-    iPvs (step_load _ _ _ j (K ++ [StoreRCtx (LocV _); FoldCtx;
+    iPvs (step_load _ _ j (K ++ [StoreRCtx (LocV _); FoldCtx;
                                    InjRCtx; PairRCtx _])
                     _ _ _ with "[Hj Hx]") as "[Hj Hx]"; eauto.
     rewrite ?fill_app. simpl.
     iFrame "Hspec Hj"; trivial.
     rewrite ?fill_app. simpl.
-    iPvs (step_store _ _ _ j K _ _ _ _ _ with "[Hj Hx]") as "[Hj Hx]"; eauto.
+    iPvs (step_store _ _ j K _ _ _ _ _ with "[Hj Hx]") as "[Hj Hx]"; eauto.
     iFrame "Hspec Hj"; trivial.
     iPvsIntro. by iFrame.
     Unshelve.
@@ -131,15 +131,15 @@ Section CG_Stack.
     (CG_locked_push st l).[f] = CG_locked_push st.[f] l.[f].
   Proof. by rewrite with_lock_subst CG_push_subst. Qed.
 
-  Lemma steps_CG_locked_push N E ρ j K st w v l :
-    nclose N ⊆ E →
-    Spec_ctx N ρ ★ st ↦ₛ v ★ l ↦ₛ (♭v false)
+  Lemma steps_CG_locked_push E ρ j K st w v l :
+    nclose specN ⊆ E →
+    spec_ctx ρ ★ st ↦ₛ v ★ l ↦ₛ (♭v false)
       ★ j ⤇ fill K (App (CG_locked_push (Loc st) (Loc l)) (# w))
     ={E}=> j ⤇ fill K Unit ★ st ↦ₛ FoldV (InjRV (PairV w v)) ★ l ↦ₛ (♭v false).
   Proof.
     intros HNE. iIntros "[#Hspec [Hx [Hl Hj]]]". unfold CG_locked_push.
     iPvs (steps_with_lock
-            _ _ _ j K _ _ _ _ UnitV _ _ _ with "[Hj Hx Hl]") as "Hj"; last done.
+            _ _ j K _ _ _ _ UnitV _ _ _ with "[Hj Hx Hl]") as "Hj"; last done.
     - iIntros {K'} "[#Hspec [Hx Hj]]".
       iApply steps_CG_push; first done. iFrame "Hspec Hj Hx"; trivial.
     - iFrame "Hspec Hj Hx"; trivial.
@@ -167,44 +167,44 @@ Section CG_Stack.
 
   Lemma CG_pop_closed (st : expr) :
     (∀ f, st.[f] = st) → ∀ f, (CG_pop st).[f] = CG_pop st.
-  Proof. intros H f. unfold CG_pop. asimpl. rewrite ?H; trivial. Qed.
+  Proof. intros Hst f. unfold CG_pop. asimpl. rewrite ?Hst; trivial. Qed.
 
   Lemma CG_pop_subst (st : expr) f : (CG_pop st).[f] = CG_pop st.[f].
   Proof. unfold CG_pop; asimpl; trivial. Qed.
 
-  Lemma steps_CG_pop_suc N E ρ j K st v w :
-    nclose N ⊆ E →
-    Spec_ctx N ρ ★ st ↦ₛ FoldV (InjRV (PairV w v)) ★
+  Lemma steps_CG_pop_suc E ρ j K st v w :
+    nclose specN ⊆ E →
+    spec_ctx ρ ★ st ↦ₛ FoldV (InjRV (PairV w v)) ★
                j ⤇ fill K (App (CG_pop (Loc st)) Unit)
       ={E}=> j ⤇ fill K (InjR (# w)) ★ st ↦ₛ v.
   Proof.
     intros HNE. iIntros "[#Hspec [Hx Hj]]". unfold CG_pop.
-    iPvs (step_lam _ _ _ j K _ _ _ _ with "[Hj]") as "Hj"; eauto.
+    iPvs (step_lam _ _ j K _ _ _ _ with "[Hj]") as "Hj"; eauto.
     asimpl.
-    iPvs (step_load _ _ _ j (K ++ [CaseCtx _ _; UnfoldCtx])
+    iPvs (step_load _ _ j (K ++ [CaseCtx _ _; UnfoldCtx])
                     _ _ _ with "[Hj Hx]") as "[Hj Hx]"; eauto.
     rewrite ?fill_app. simpl.
     iFrame "Hspec Hj"; trivial.
     rewrite ?fill_app. simpl.
-    iPvs (step_Fold _ _ _ j (K ++ [CaseCtx _ _])
+    iPvs (step_Fold  _ _ j (K ++ [CaseCtx _ _])
                     _ _ _ _ with "[Hj]") as "Hj"; eauto.
     rewrite ?fill_app. simpl.
     iFrame "Hspec Hj"; trivial.
     rewrite ?fill_app. simpl.
-    iPvs (step_case_inr _ _ _ j K _ _ _ _ _ with "[Hj]") as "Hj"; eauto.
+    iPvs (step_case_inr _ _ j K _ _ _ _ _ with "[Hj]") as "Hj"; eauto.
     asimpl.
-    iPvs (step_snd _ _ _ j (K ++ [AppRCtx (LamV _); StoreRCtx (LocV _)]) _ _ _ _
+    iPvs (step_snd _ _ j (K ++ [AppRCtx (LamV _); StoreRCtx (LocV _)]) _ _ _ _
                    _ _ with "[Hj]") as "Hj"; eauto.
     rewrite ?fill_app. simpl.
     iFrame "Hspec Hj"; trivial.
-    iPvs (step_store _ _ _ j (K ++ [AppRCtx (LamV _)]) _ _ _ _ _ _
+    iPvs (step_store _ _ j (K ++ [AppRCtx (LamV _)]) _ _ _ _ _ _
           with "[Hj Hx]") as "[Hj Hx]"; eauto.
     rewrite ?fill_app. simpl.
     iFrame "Hspec Hj"; trivial.
     rewrite ?fill_app. simpl.
-    iPvs (step_lam _ _ _ j K _ _ _ _ with "[Hj]") as "Hj"; eauto.
+    iPvs (step_lam _ _ j K _ _ _ _ with "[Hj]") as "Hj"; eauto.
     asimpl.
-    iPvs (step_fst _ _ _ j (K ++ [InjRCtx]) _ _ _ _ _ _
+    iPvs (step_fst _ _ j (K ++ [InjRCtx]) _ _ _ _ _ _
           with "[Hj]") as "Hj"; eauto.
     rewrite ?fill_app. simpl.
     iFrame "Hspec Hj"; trivial. asimpl.
@@ -215,26 +215,26 @@ Section CG_Stack.
     all: trivial.
   Qed.
 
-  Lemma steps_CG_pop_fail N E ρ j K st :
-    nclose N ⊆ E →
-    Spec_ctx N ρ ★ st ↦ₛ FoldV (InjLV UnitV) ★
+  Lemma steps_CG_pop_fail E ρ j K st :
+    nclose specN ⊆ E →
+    spec_ctx ρ ★ st ↦ₛ FoldV (InjLV UnitV) ★
                j ⤇ fill K (App (CG_pop (Loc st)) Unit)
       ={E}=> j ⤇ fill K (InjL Unit) ★ st ↦ₛ FoldV (InjLV UnitV).
   Proof.
     iIntros {HNE} "[#Hspec [Hx Hj]]". unfold CG_pop.
-    iPvs (step_lam _ _ _ j K _ _ _ _ with "[Hj]") as "Hj"; eauto.
+    iPvs (step_lam _ _ j K _ _ _ _ with "[Hj]") as "Hj"; eauto.
     asimpl.
-    iPvs (step_load _ _ _ j (K ++ [CaseCtx _ _; UnfoldCtx])
+    iPvs (step_load _ _ j (K ++ [CaseCtx _ _; UnfoldCtx])
                     _ _ _ with "[Hj Hx]") as "[Hj Hx]"; eauto.
     rewrite ?fill_app. simpl.
     iFrame "Hspec Hj"; trivial.
     rewrite ?fill_app. simpl.
-    iPvs (step_Fold _ _ _ j (K ++ [CaseCtx _ _])
+    iPvs (step_Fold _ _ j (K ++ [CaseCtx _ _])
                     _ _ _ _ with "[Hj]") as "Hj"; eauto.
     rewrite ?fill_app. simpl.
     iFrame "Hspec Hj"; trivial.
     rewrite ?fill_app. simpl.
-    iPvs (step_case_inl _ _ _ j K _ _ _ _ _ with "[Hj]") as "Hj"; eauto.
+    iPvs (step_case_inl _ _ j K _ _ _ _ _ with "[Hj]") as "Hj"; eauto.
     asimpl.
     iPvsIntro. iFrame "Hj Hx"; trivial.
     Unshelve.
@@ -275,14 +275,14 @@ Section CG_Stack.
   (CG_locked_pop st l).[f] = CG_locked_pop st.[f] l.[f].
   Proof. by rewrite with_lock_subst CG_pop_subst. Qed.
 
-  Lemma steps_CG_locked_pop_suc N E ρ j K st v w l :
-    nclose N ⊆ E →
-    Spec_ctx N ρ ★ st ↦ₛ FoldV (InjRV (PairV w v)) ★ l ↦ₛ (♭v false)
+  Lemma steps_CG_locked_pop_suc E ρ j K st v w l :
+    nclose specN ⊆ E →
+    spec_ctx ρ ★ st ↦ₛ FoldV (InjRV (PairV w v)) ★ l ↦ₛ (♭v false)
                ★ j ⤇ fill K (App (CG_locked_pop (Loc st) (Loc l)) Unit)
       ={E}=> j ⤇ fill K (InjR (# w)) ★ st ↦ₛ v ★ l ↦ₛ (♭v false).
   Proof.
     iIntros {HNE} "[#Hspec [Hx [Hl Hj]]]". unfold CG_locked_pop.
-    iPvs (steps_with_lock _ _ _ j K _ _ _ _ (InjRV w) UnitV _ _
+    iPvs (steps_with_lock _ _ j K _ _ _ _ (InjRV w) UnitV _ _
           with "[Hj Hx Hl]") as "Hj"; last done.
     - iIntros {K'} "[#Hspec [Hx Hj]]".
       iApply steps_CG_pop_suc; first done. iFrame "Hspec Hj Hx"; trivial.
@@ -290,14 +290,14 @@ Section CG_Stack.
       Unshelve. all: trivial.
   Qed.
 
-  Lemma steps_CG_locked_pop_fail N E ρ j K st l :
-    nclose N ⊆ E →
-    Spec_ctx N ρ ★ st ↦ₛ FoldV (InjLV UnitV) ★ l ↦ₛ (♭v false)
+  Lemma steps_CG_locked_pop_fail E ρ j K st l :
+    nclose specN ⊆ E →
+    spec_ctx ρ ★ st ↦ₛ FoldV (InjLV UnitV) ★ l ↦ₛ (♭v false)
                ★ j ⤇ fill K (App (CG_locked_pop (Loc st) (Loc l)) Unit)
       ={E}=> j ⤇ fill K (InjL Unit) ★ st ↦ₛ FoldV (InjLV UnitV) ★ l ↦ₛ (♭v false).
   Proof.
     iIntros {HNE} "[#Hspec [Hx [Hl Hj]]]". unfold CG_locked_pop.
-    iPvs (steps_with_lock _ _ _ j K _ _ _ _ (InjLV UnitV) UnitV _ _
+    iPvs (steps_with_lock _ _ j K _ _ _ _ (InjLV UnitV) UnitV _ _
           with "[Hj Hx Hl]") as "Hj"; last done.
     - iIntros {K'} "[#Hspec [Hx Hj]]". simpl.
       iApply steps_CG_pop_fail; first done. iFrame "Hspec Hj Hx"; trivial.
@@ -338,19 +338,19 @@ Section CG_Stack.
     (CG_snap st l).[f] = CG_snap st.[f] l.[f].
   Proof. unfold CG_snap; rewrite ?with_lock_subst. by asimpl. Qed.
 
-  Lemma steps_CG_snap N E ρ j K st v l :
-    nclose N ⊆ E →
-    Spec_ctx N ρ ★ st ↦ₛ v ★ l ↦ₛ (♭v false)
+  Lemma steps_CG_snap E ρ j K st v l :
+    nclose specN ⊆ E →
+    spec_ctx ρ ★ st ↦ₛ v ★ l ↦ₛ (♭v false)
                ★ j ⤇ fill K (App (CG_snap (Loc st) (Loc l)) Unit)
       ={E}=> j ⤇ (fill K (# v)) ★ st ↦ₛ v ★ l ↦ₛ (♭v false).
   Proof.
     iIntros {HNE} "[#Hspec [Hx [Hl Hj]]]". unfold CG_snap.
-    iPvs (steps_with_lock _ _ _ j K _ _ _ _ v UnitV _ _
+    iPvs (steps_with_lock _ _ j K _ _ _ _ v UnitV _ _
           with "[Hj Hx Hl]") as "Hj"; last done; [|by iFrame "Hspec Hx Hl Hj"].
     iIntros {K'} "[#Hspec [Hx Hj]]".
-    iPvs (step_lam _ _ _ j K' _ _ _ _ with "[Hj]") as "Hj"; eauto.
+    iPvs (step_lam _ _ j K' _ _ _ _ with "[Hj]") as "Hj"; eauto.
     asimpl.
-    iPvs (step_load _ _ _ j K' _ _ _ _
+    iPvs (step_load _ _ j K' _ _ _ _
           with "[Hj Hx]") as "[Hj Hx]"; eauto.
     - by iFrame "Hspec Hj Hx".
     - iPvsIntro. by iFrame "Hj Hx".
@@ -398,14 +398,14 @@ Section CG_Stack.
 
   Lemma CG_iter_closed (f : expr) :
     (∀ g, f.[g] = f) → ∀ g, (CG_iter f).[g] = CG_iter f.
-  Proof. intros H g. unfold CG_iter. asimpl. rewrite ?H; trivial. Qed.
+  Proof. intros Hf g. unfold CG_iter. asimpl. rewrite ?Hf; trivial. Qed.
 
   Lemma CG_iter_subst (f : expr) g : (CG_iter f).[g] = CG_iter f.[g].
   Proof. unfold CG_iter; asimpl; trivial. Qed.
 
-  Lemma steps_CG_iter N E ρ j K f v w :
-    nclose N ⊆ E →
-    Spec_ctx N ρ
+  Lemma steps_CG_iter E ρ j K f v w :
+    nclose specN ⊆ E →
+    spec_ctx ρ
         ★ j ⤇ fill K (App (CG_iter (# f)) (Fold (InjR (Pair (# w) (# v)))))
       ={E}=>
     j ⤇ fill K
@@ -416,16 +416,16 @@ Section CG_Stack.
              (App (# f) (# w))).
   Proof.
     iIntros {HNE} "[#Hspec Hj]". unfold CG_iter.
-    iPvs (step_lam _ _ _ j K _ _ _ _ with "[Hj]") as "Hj"; eauto.
+    iPvs (step_lam _ _ j K _ _ _ _ with "[Hj]") as "Hj"; eauto.
     rewrite -CG_iter_folding. Opaque CG_iter. asimpl.
-    iPvs (step_Fold _ _ _ j (K ++ [CaseCtx _ _])
+    iPvs (step_Fold _ _ j (K ++ [CaseCtx _ _])
                     _ _ _ with "[Hj]") as "Hj"; eauto.
     rewrite ?fill_app /=.
     iFrame "Hspec Hj"; trivial.
     rewrite ?fill_app. asimpl.
-    iPvs (step_case_inr _ _ _ j K _ _ _ _ _ with "[Hj]") as "Hj"; eauto.
+    iPvs (step_case_inr _ _ j K _ _ _ _ _ with "[Hj]") as "Hj"; eauto.
     asimpl.
-    iPvs (step_fst _ _ _ j (K ++ [AppRCtx (LamV _); AppRCtx f]) _ _ _ _
+    iPvs (step_fst _ _ j (K ++ [AppRCtx (LamV _); AppRCtx f]) _ _ _ _
                    _ _ with "[Hj]") as "Hj"; eauto.
     rewrite ?fill_app /=.
     iFrame "Hspec Hj"; trivial.
@@ -437,20 +437,20 @@ Section CG_Stack.
 
   Transparent CG_iter.
 
-  Lemma steps_CG_iter_end N E ρ j K f :
-    nclose N ⊆ E →
-    Spec_ctx N ρ ★ j ⤇ fill K (App (CG_iter (# f)) (Fold (InjL Unit)))
+  Lemma steps_CG_iter_end E ρ j K f :
+    nclose specN ⊆ E →
+    spec_ctx ρ ★ j ⤇ fill K (App (CG_iter (# f)) (Fold (InjL Unit)))
       ={E}=> j ⤇ fill K Unit.
   Proof.
     iIntros {HNE} "[#Hspec Hj]". unfold CG_iter.
-    iPvs (step_lam _ _ _ j K _ _ _ _ with "[Hj]") as "Hj"; eauto.
+    iPvs (step_lam _ _ j K _ _ _ _ with "[Hj]") as "Hj"; eauto.
     rewrite -CG_iter_folding. Opaque CG_iter. asimpl.
-    iPvs (step_Fold _ _ _ j (K ++ [CaseCtx _ _])
+    iPvs (step_Fold _ _ j (K ++ [CaseCtx _ _])
                     _ _ _ with "[Hj]") as "Hj"; eauto.
     rewrite ?fill_app /=.
     iFrame "Hspec Hj"; trivial.
     rewrite ?fill_app. asimpl.
-    iPvs (step_case_inl _ _ _ j K _ _ _ _ _ with "[Hj]") as "Hj"; eauto.
+    iPvs (step_case_inl _ _ j K _ _ _ _ _ with "[Hj]") as "Hj"; eauto.
     Unshelve.
     all: try match goal with |- to_val _ = _ => simpl; by rewrite ?to_of_val end.
   Qed.
